ViperBoogieEndToEnd.thy
@@ -2,16 +2,6 @@ theory ViperBoogieEndToEnd
 imports StmtRel
 begin
 
-definition vpr_method_correct_total :: "'a total_context \<Rightarrow> ('a full_total_state \<Rightarrow> bool) \<Rightarrow> method_decl \<Rightarrow> bool" where
-  "vpr_method_correct_total ctxt R mdecl \<equiv>
-        \<forall>mbody. method_decl.body mdecl = Some mbody \<longrightarrow>
-         (\<forall>(\<omega> :: 'a full_total_state) r. 
-                  \<comment>\<open>TODO: reverse list?\<close>
-                  vpr_store_well_typed (absval_interp_total ctxt) (nth_option (method_decl.args mdecl @ method_decl.rets mdecl)) (get_store_total \<omega>) \<longrightarrow>
-                  total_heap_well_typed (program_total ctxt) (absval_interp_total ctxt) (get_hh_total_full \<omega>) \<longrightarrow>
-                  is_empty_total_full \<omega> \<longrightarrow>
-                  red_stmt_total ctxt R (nth_option (method_decl.args mdecl @ method_decl.rets mdecl)) mbody \<omega> r \<longrightarrow> r \<noteq> RFailure)"
-
 text \<open>Accesses to old expressions are represented via labeled old expressions with label \<^const>\<open>old_label\<close>.\<close>  
 
 lemma valid_configuration_not_failure:
@@ -215,165 +205,6 @@ lemma proc_body_satisfies_spec_valid_config:
   unfolding proc_body_satisfies_spec_def
   by blast
 
-lemma end_to_end_stmt_rel:
-  assumes 
-          \<comment>\<open>The Boogie procedure is correct.\<close>             
-             \<comment>\<open>Note that we need to explicitly provide the type for term\<open>A\<close> to 
-                be able to instantiate A with \<^term>\<open>vbpl_absval_ty TyRep\<close>\<close>
-          Boogie_correct: "proc_is_correct (vbpl_absval_ty (TyRep :: 'a ty_repr_bpl)) fun_decls constants global_vars axioms (proc_bpl :: ast procedure) 
-                  (Ast.proc_body_satisfies_spec :: (('a vbpl_absval, ast) proc_body_satisfies_spec_ty))" and 
-
-          VprMethodBodySome: "method_decl.body mdecl = Some body_vpr" and
-
-          ProcBodySome: "proc_body proc_bpl = Some (locals_bpl, proc_body_bpl)" and
-
-          \<comment>\<open>Viper encoding does not use Boogie procedure preconditions\<close>
-          ProcPresEmpty: "proc_pres proc_bpl = []" and
-                         "\<Lambda> = (nth_option (method_decl.args mdecl @ rets mdecl))" and
-          \<comment>\<open>Viper and Boogie statement are related\<close>
-          StmtRel: "stmt_rel 
-             \<comment>\<open>input relation\<close>
-             (state_rel_empty (state_rel_well_def_same ctxt Pr StateCons (TyRep :: 'a ty_repr_bpl) Tr AuxPred))
-             \<comment>\<open>output relation is irrelevant\<close>
-             R' 
-             ctxt_vpr StateCons \<Lambda> proc_body_bpl ctxt 
-             body_vpr 
-             \<comment>\<open>initial program point in Boogie procedure body\<close>
-             (convert_ast_to_program_point proc_body_bpl)
-             \<comment>\<open>output program point in Boogie procedure body is irrelevant\<close>
-             \<gamma>'"  and 
-    TypeInterpEq: "type_interp ctxt = vbpl_absval_ty TyRep" and                  
-    ProcTyArgsEmpty: "proc_ty_args proc_bpl = 0" "rtype_interp ctxt = []" and
-    VarCtxtEq: "var_context ctxt = (constants @ global_vars, proc_args proc_bpl @ locals_bpl @ proc_rets proc_bpl)" and
-    WfTyRep: "wf_ty_repr_bpl TyRep" and
-\<comment>\<open>TODO: I have not yet proved the following assumptions for specific Boogie programs\<close>
-     FunInterp: "fun_interp_wf (vbpl_absval_ty TyRep) fun_decls (fun_interp ctxt)" and
-     InitialStateRel: "\<And> \<omega>.  
-                       vpr_store_well_typed (absval_interp_total ctxt_vpr) (nth_option (method_decl.args mdecl @ rets mdecl)) (get_store_total \<omega>) \<Longrightarrow>
-                       total_heap_well_typed (program_total ctxt_vpr) (absval_interp_total ctxt_vpr) (get_hh_total_full \<omega>) \<Longrightarrow>
-                       is_empty_total_full \<omega> \<Longrightarrow>
-                       \<exists>ns ls gs.
-                           ns = \<lparr>old_global_state = gs, global_state = gs, local_state = ls, binder_state = Map.empty\<rparr> \<and>  
-                           \<comment>\<open>well-typedness of Boogie state follows from state relation\<close>
-                           (state_rel_empty (state_rel_well_def_same ctxt Pr StateCons (TyRep :: 'a ty_repr_bpl) Tr AuxPred)) \<omega> ns \<and>
-                           axioms_sat (vbpl_absval_ty TyRep) (constants, []) (fun_interp ctxt) (global_to_nstate (state_restriction gs constants)) axioms"
-shows "vpr_method_correct_total ctxt_vpr StateCons mdecl"
-  unfolding vpr_method_correct_total_def
-proof (rule allI | rule impI)+
-  let ?\<Lambda> = "(nth_option (method_decl.args mdecl @ rets mdecl))"
-  fix \<omega> r  body_vpr_prf
-  assume "method_decl.body mdecl = Some body_vpr_prf" and
-         StoreWellTy: "vpr_store_well_typed (absval_interp_total ctxt_vpr) (nth_option (method_decl.args mdecl @ rets mdecl)) (get_store_total \<omega>)" and
-         HeapWellTy: "total_heap_well_typed (program_total ctxt_vpr) (absval_interp_total ctxt_vpr) (get_hh_total_full \<omega>)" and
-         "is_empty_total_full \<omega>" and
-         RedStmtVpr:"red_stmt_total ctxt_vpr StateCons ?\<Lambda> body_vpr_prf \<omega> r"
-
-  hence "body_vpr_prf = body_vpr"
-    using VprMethodBodySome
-    by simp
-  
-  let ?abs="vbpl_absval_ty TyRep"
-
-  note Boogie_correct_inst=Boogie_correct
-
-  obtain ns ls gs where 
-    "ns = \<lparr>old_global_state = gs, global_state = gs, local_state = ls, binder_state = Map.empty\<rparr>" and
-  StateRelInitialInst: 
-    "state_rel_empty (state_rel_well_def_same ctxt Pr StateCons (TyRep :: 'a ty_repr_bpl) Tr AuxPred) \<omega> ns" and
-  AxiomsSat:
-    "axioms_sat (vbpl_absval_ty TyRep) (constants, []) (fun_interp ctxt) (global_to_nstate (state_restriction gs constants)) axioms"
-    using InitialStateRel[OF StoreWellTy HeapWellTy \<open>is_empty_total_full \<omega>\<close>]
-    by blast
-
-  from StateRelInitialInst have StateRel: "state_rel Pr StateCons TyRep Tr AuxPred ctxt \<omega> \<omega> ns"
-    by (simp add: state_rel_empty_def)
-    
-  have
-    GlobalsWf: "state_typ_wf (vbpl_absval_ty TyRep) [] gs (constants @ global_vars)" and
-    LocalsWf: "state_typ_wf (vbpl_absval_ty TyRep) [] ls ((proc_args proc_bpl)@ (locals_bpl @ proc_rets proc_bpl))"
-    using state_rel_state_well_typed[OF StateRel] \<open>ns = _\<close> VarCtxtEq TypeInterpEq
-    unfolding state_rel_empty_def state_well_typed_def 
-    by auto          
-  
-  have ProcBodyBplCorrect:
-      "(Ast.proc_body_satisfies_spec :: (('a vbpl_absval, ast) proc_body_satisfies_spec_ty)) ?abs [] (constants@global_vars, (proc_args proc_bpl)@(locals_bpl@(proc_rets proc_bpl))) (fun_interp ctxt) [] 
-                                       (proc_all_pres proc_bpl) (proc_checked_posts proc_bpl) proc_body_bpl
-                                       \<lparr>old_global_state = gs, global_state = gs, local_state = ls, binder_state = Map.empty\<rparr>"
-  proof (rule proc_is_correct_elim[OF Boogie_correct_inst ProcBodySome])
-    show "\<forall>t. closed t \<longrightarrow> (\<exists>v. type_of_vbpl_val TyRep v = t)"
-      by (simp add: closed_types_inhabited)
-  next
-    show "\<forall>v. closed (type_of_vbpl_val TyRep v)"
-    proof (rule allI)
-      fix v
-      show "closed (type_of_vbpl_val TyRep v)"
-      proof (cases v)
-        case (LitV x1)
-        then show ?thesis by simp
-      next
-        case (AbsV x2)
-        then show ?thesis 
-          using vbpl_absval_ty_closed[OF WfTyRep]
-          by fastforce
-      qed
-    qed
-  next
-    show "fun_interp_wf (vbpl_absval_ty TyRep) fun_decls (fun_interp ctxt)"
-      by (rule FunInterp)
-  next
-    show "list_all closed [] \<and> length []  = proc_ty_args proc_bpl"
-      by (simp add: ProcTyArgsEmpty)
-  next
-    show "state_typ_wf (vbpl_absval_ty TyRep) [] gs (constants @ global_vars)"
-      by (rule GlobalsWf)
-  next 
-    show "state_typ_wf (vbpl_absval_ty TyRep) [] ls (proc_args proc_bpl @ locals_bpl @ proc_rets proc_bpl)"
-      by (rule LocalsWf)
-  next
-    show "axioms_sat (vbpl_absval_ty TyRep) (constants, []) (fun_interp ctxt) (global_to_nstate (state_restriction gs constants)) axioms"
-      by (rule AxiomsSat)
-  qed
-
-  show "r \<noteq> RFailure"
-  proof (rule ccontr)
-    assume "\<not> r \<noteq> RFailure"
-    hence "r = RFailure" by simp
-
-    from stmt_rel_failure_elim[OF StmtRel StateRelInitialInst] RedStmtVpr \<open>r = _\<close> obtain c' where
-     FailureConfig: "snd c' = Failure" and 
-      RedBpl: "red_ast_bpl proc_body_bpl ctxt (convert_ast_to_program_point proc_body_bpl, Normal ns) c'"
-      using \<open>body_vpr_prf = _\<close> \<open>\<Lambda> = _\<close>
-      by blast
-
-    let ?c'_program_point = "fst c'"
-    let ?c'_bigblock = "fst ?c'_program_point"
-    let ?c'_cont = "snd ?c'_program_point"
-
-    obtain d' where 
-      RedBigBlockMulti: "(red_bigblock_multi (vbpl_absval_ty TyRep) ([] :: ast proc_context) (constants @ global_vars, proc_args proc_bpl @ locals_bpl @ proc_rets proc_bpl) (fun_interp ctxt) [] proc_body_bpl)\<^sup>*\<^sup>*
-         (init_ast proc_body_bpl \<lparr>old_global_state = gs, global_state = gs, local_state = ls, binder_state = Map.empty\<rparr>) d'" and
-      "snd (snd d') = Failure"
-
-      using red_ast_block_red_bigblock_failure_preserve[OF RedBpl FailureConfig TypeInterpEq VarCtxtEq HOL.refl]
-            \<open>ns = _\<close> ProcTyArgsEmpty
-      by (auto simp: init_ast_convert_ast_to_program_point_eq)
-    
-    let ?d'_bigblock = "fst d'"
-    let ?d'_cont = "fst (snd d')"
-    let ?d'_state = "snd (snd d')"
-
-    have "Ast.valid_configuration (vbpl_absval_ty TyRep) (constants @ global_vars, proc_args proc_bpl @ locals_bpl @ proc_rets proc_bpl)
-         (fun_interp ctxt) [] (Ast.proc_checked_posts proc_bpl) ?d'_bigblock ?d'_cont ?d'_state"
-      apply (rule proc_body_satisfies_spec_valid_config[OF ProcBodyBplCorrect] )
-      using ProcPresEmpty RedBigBlockMulti
-      unfolding expr_all_sat_def
-      by auto
-    thus False
-      using \<open>snd (snd d') = Failure\<close> valid_configuration_not_failure
-      by blast    
-  qed
-qed
-
 text\<open>\<^const>\<open>Ast.proc_body_satisfies_spec\<close> is expressed via \<^const>\<open>red_bigblock\<close>, while \<^const>\<open>red_ast_bpl\<close> 
      is expressed via \<^const>\<open>red_bigblock_small\<close>. The following lemma bridges the gap.\<close>
 
@@ -464,11 +295,6 @@ lemma post_framing_rel_aux:
                               (range (const_repr Tr)) \<union>
                               dom AuxPred) = {}" (is "?A \<inter> ?B = {}")
       and "hvar' \<noteq> mvar'"
-     (* and PropagateBpl: "\<And> \<omega>0 ns. (state_rel_well_def_same ctxt Pr StateCons (TyRep :: 'a ty_repr_bpl) Tr AuxPred) \<omega>0 ns \<Longrightarrow>
-                            \<exists>ns'. red_ast_bpl proc_body_bpl ctxt 
-                                    (\<gamma>Pre, Normal ns)
-                                    ((BigBlock name (Havoc hvar' # Assign mvar' (Var zero_mask_var) # cs) str tr, cont), Normal ns') \<and>
-                               (state_rel_well_def_same ctxt Pr StateCons (TyRep :: 'a ty_repr_bpl) Tr AuxPred) \<omega>0 ns'"*)
       and PropagateBpl: "red_ast_bpl_rel (state_rel_well_def_same ctxt Pr StateCons (TyRep :: 'a ty_repr_bpl) Tr AuxPred) 
                                          (state_rel_well_def_same ctxt Pr StateCons (TyRep :: 'a ty_repr_bpl) Tr AuxPred) proc_body_bpl ctxt 
                                          \<gamma>Pre 
@@ -554,7 +380,7 @@ definition vpr_method_correct_total_partial :: "'a total_context \<Rightarrow> (
 lemma vpr_method_correct_total_from_partial:
   assumes "\<And> m' mdecl' . methods (program_total ctxt) m' = Some mdecl' \<Longrightarrow> vpr_method_correct_total_partial ctxt StateCons mdecl'"
       and "methods (program_total ctxt) m = Some mdecl"
-    shows  "vpr_method_correct_total_2_new ctxt StateCons mdecl"
+    shows "vpr_method_correct_total ctxt StateCons mdecl"
 proof -
   have SpecsCorrect: "vpr_all_method_spec_correct_total ctxt StateCons (program_total ctxt)"
     unfolding vpr_all_method_spec_correct_total_def
@@ -573,13 +399,13 @@ proof -
     using assms
     by auto
 
-  thus "vpr_method_correct_total_2_new ctxt StateCons mdecl"
+  thus "vpr_method_correct_total ctxt StateCons mdecl"
     using SpecsCorrect
-    unfolding vpr_method_correct_total_partial_def vpr_method_correct_total_2_new_def vpr_method_correct_total_aux_def
+    unfolding vpr_method_correct_total_partial_def vpr_method_correct_total_def vpr_method_correct_total_aux_def
     by blast
 qed
 
-lemma end_to_end_stmt_rel_2:
+lemma end_to_end_vpr_method_correct_partial:
   assumes 
           \<comment>\<open>The Boogie procedure is correct. Note that we need to explicitly provide the types such that
              we can then instantiate the Boogie type interpretation with \<^term>\<open>vbpl_absval_ty TyRep\<close>.\<close>
@@ -588,8 +414,8 @@ lemma end_to_end_stmt_rel_2:
       and ConsistencyDownwardMono: "mono_prop_downward_ord StateCons"
       and ProgMethod: "methods (program_total ctxt_vpr) mname = Some mdecl"
       and VprMethodBodySome: "method_decl.body mdecl = Some body_vpr"
-      and VprNoPermUnfoldingPre: "no_perm_assertion (method_decl.pre mdecl) \<and> no_unfolding_assertion (method_decl.pre mdecl)"
-      and VprNoPermUnfoldingPost: "no_perm_assertion (method_decl.post mdecl) \<and> no_unfolding_assertion (method_decl.post mdecl)"
+      and VprNoPermUnfoldingSpec: "no_perm_assertion (method_decl.pre mdecl) \<and> no_unfolding_assertion (method_decl.pre mdecl) \<and>
+                                   no_perm_assertion (method_decl.post mdecl) \<and> no_unfolding_assertion (method_decl.post mdecl)"
       and OnlyArgsInPre: "\<And> x. x \<in> free_var_assertion (method_decl.pre mdecl) \<Longrightarrow> x < length (method_decl.args mdecl)"
       and ArgsAndRetsUnmodified: "\<And>x. x < (length (method_decl.args mdecl) + length (method_decl.rets mdecl)) \<Longrightarrow> x \<notin> modif body_vpr"
       and ProcBodySome: "proc_body proc_bpl = Some (locals_bpl, proc_body_bpl)"
@@ -791,7 +617,7 @@ proof (rule allI | rule impI)+
 
           with inhale_no_perm_downwards_mono(3) ConsistencyDownwardMono  RedInhPost 
           have "red_inhale ctxt_vpr StateCons (method_decl.post mdecl) ?\<omega>PostEmpty RFailure"
-            using is_empty_empty_full_total_state \<open>res = _\<close>  VprNoPermUnfoldingPost
+            using is_empty_empty_full_total_state \<open>res = _\<close>  VprNoPermUnfoldingSpec
             by blast
             
           with stmt_rel_failure_elim[OF PostFramingInhRel \<open>RPostFrameStart _ _\<close>]
@@ -915,7 +741,7 @@ proof (rule allI | rule impI)+
                   by simp           
               qed                
 
-              with OnlyArgsInPre VprNoPermUnfoldingPre RedInhPre \<open>rpre = RNormal \<omega>pre\<close>
+              with OnlyArgsInPre VprNoPermUnfoldingSpec RedInhPre \<open>rpre = RNormal \<omega>pre\<close>
               have RedInhStoreBody: "red_inhale ctxt_vpr StateCons (method_decl.pre mdecl) 
                         ?\<omega>_store_body (RNormal (\<omega>pre \<lparr> get_store_total := get_store_total \<omega>body \<rparr>))"
                 using red_pure_exp_inhale_store_same_on_free_var(3)[OF RedInhPre _ StoresAgreeOnArgs]
